update list demo, add is_z test, rename wf tactic

tests/Lists.v
@@ -17,486 +17,411 @@ Require Import Coq.Strings.String.
 Require Import MirrorSolve.Reflection.Core.
 Require Import MirrorSolve.Reflection.FM.
 
+Require Import Coq.ZArith.BinInt.
+
+(* In this demo we make two different versions of list reverse:
+  1) my_rev, which is a naive quadratic list reverse (it uses append at each step, which is linear, on each element of the input)
+  2) tail_rev, which is a classic tail-optimized linear list reverse.
+
+  We prove that forall xs, my_rev xs = tail_rev xs using mirrorsolve's proof automation
+
+  To demo the rest of mirrorsolve, we also define a length function, and a custom predicate, and prove properties about them with reverse.
+*)
+
 Section ListFuncs.
   Variable (A: Type).
 
-  Fixpoint app (l: list A) (r: list A) := 
-    match l with 
-    | nil => r
-    | x :: l' => x :: app l' r
-    end.
+  (* We will make use of a hint database to reflect recursive coq functions into SMT logic.
+     For now, don't worry about it, but it's handy to use Equations for recursion to make use of the generated equations.
+   *)
 
-  Lemma app_nil: 
-    forall xs, 
-      app nil xs = xs.
-  Proof.
-    intros; exact eq_refl.
-  Qed.
+  Equations my_app (l: list A) (r: list A) : list A := {
+    my_app nil r := r;
+    my_app (x :: l') r := x :: my_app l' r;
+  }.
 
-  Lemma app_cons: 
-    forall x xs ys, 
-      app (x :: xs) ys = x :: (app xs ys).
-  Proof.
-    intros; exact eq_refl.
-  Qed.
-
-  Fixpoint my_rev (xs: list A) :=
-    match xs with 
-    | nil => nil
-    | x :: xs' => app (my_rev xs') [x]
-    end. 
-
-  Lemma my_rev_nil: 
-    my_rev nil = nil.
-  Proof.
-    intros; exact eq_refl.
-  Qed.
-
-  Lemma my_rev_cons: 
-    forall x xs, 
-      my_rev (x :: xs) = app (my_rev xs) [x].
-  Proof.
-    intros; exact eq_refl.
-  Qed.
-
-  Fixpoint tail_app (acc: list A) (l_rev: list A) : list A := 
-    match l_rev with 
-    | nil => acc
-    | (l :: l_rev') => tail_app (l :: acc) l_rev'
-    end. 
-
-  Lemma tail_app_nil: 
-    forall acc, 
-      tail_app acc nil = acc.
-  Proof.
-    intros; exact eq_refl.
-  Qed.
-
-  Lemma tail_app_cons: 
-    forall acc x xs, 
-      tail_app acc (x :: xs) = tail_app (x :: acc) xs.
-  Proof.
-    intros; exact eq_refl.
-  Qed.
+  Check my_app_equation_1. (* forall r : list A, my_app [] r = r *)
+  Check my_app_equation_2. (* forall (x : A) (l' r : list A), my_app (x :: l') r = x :: my_app l' r *)
   
-  Definition my_app l r := tail_app r (my_rev l).
+  Equations my_rev (xs: list A) : list A := {
+    my_rev nil := nil;
+    my_rev (x :: l') := my_app (my_rev l') [x];
+  }.
 
-  From Hammer Require Import Hammer.
+  Equations tail_rev (xs: list A) (acc: list A) : list A := {
+    tail_rev nil acc := acc;
+    tail_rev (x :: xs') acc := tail_rev xs' (x :: acc);
+  }.
 
-  Set Hammer ATPLimit 5.
-  Set Hammer ReconstrLimit 10.
+  Equations my_In (x: A) (l: list A) : Prop := {
+    my_In x nil := False;
+    my_In x (x' :: l') := x = x' \/ my_In x l';
+  }.
 
-  (* we will model this using three UF functions, for rev, app, and tail_app *)
-
-
-  Set Universe Polymorphism.
-
-  Notation sig := FOList.sig.
-
-  Definition list_model := FOList.fm_model A.
-
-  (* First, set up uninterpreted function symbols for app, rev, and tail_rev *)
-  Definition symbs : list (string * list (sig_sorts sig) * sig_sorts sig) := ([
-    ("app", [LS; LS], LS); 
-    ("rev", [LS], LS); 
-    ("tail_app", [LS; LS], LS) 
-  ]%string).
-
-  Lemma in_conv : forall {sym a r}, 
-    In (sym, a, r) symbs -> 
-    in_symbs sig sorts_eq_dec symbs sym a r = true.
+  Lemma my_In_equation_1' : 
+    forall x, ~ my_In x [].
   Proof.
-    eapply UF.in_symbs_corr.
-  Defined.
+    intros.
+    autorewrite with my_In.
+    intuition eauto.
+  Qed.
 
-  Import HListNotations.
+  Lemma my_In_equation_2' : 
+    forall (x x' : A) (l' : list A),
+      my_In x (x' :: l') <-> (x = x' \/ my_In x l').
+  Proof.
+    intros.
+    (* simpl. *)
+    autorewrite with my_In.
+    intuition eauto.
+  Qed.
 
-  (* Interpretation function for UF symbols. 
-    In order for the reflection machinery to work out, we need to provide an actual interpretation for the UF symbols (even though they will be discharged as UF symbols in SMT).  *)
-  Definition interp_syms (sym: string) (a: list (sig_sorts sig)) (r: sig_sorts sig) (H: In (sym, a, r) symbs) (args: HList.t (FirstOrder.mod_sorts sig list_model) a) : FirstOrder.mod_sorts sig list_model r.
-    pose proof in_conv H.
-    unfold in_symbs in H0.
-    simpl in H0.
-    repeat match goal with 
-    | H: (if (?L =? ?R)%string then _ else _) = _ |- _ => 
-      destruct (comp_str_eqb_spec L R)
-    | H: (if ?A then _ else _) = _ |- _ => 
-      destruct A eqn:?
-    end; try congruence;
-    subst;
-    repeat match goal with 
-    | X: HList.t _ _ |- _ => 
-      inversion X; subst; clear X
+  (* For simplicity we use Z instead of nat or N, because Z translates directly to SMT. 
+     We could also use nat or N and use the N2Z functor to convert goals from nat/N to Z. 
+  *)
+  Equations my_len (xs: list A) : Z := {
+    my_len nil := 0;
+    my_len (_ :: xs) := my_len xs + 1;
+  }.
+
+  (* Next we set up a first-order logic for lists, my_app, my_rev, tail_rev, my_In, and my_len.
+   *)
+
+  (* First we need a syntax and semantics for sorts. Our three sorts are A, list A, and Z,
+    and we'll need a bool sort for my_In's Prop down the road. *)
+  Inductive fol_sorts := sort_A | sort_lA | sort_Z | sort_bool.
+  Definition interp_sorts (x: fol_sorts) : Type := 
+    match x with 
+    | sort_A => A
+    | sort_lA => list A
+    | sort_Z => Z
+    | sort_bool => bool
     end.
-    - exact (app X X1).
-    - exact (my_rev X).
-    - exact (tail_app X X1).
-  Defined.
 
-  Definition list_uf_model := UF.fm_model sig list_model symbs interp_syms.
+  (* Next we define function symbols for everything mentioned in the functions:
+    nil, cons, my_app, my_rev, tail_rev, my_len, Z plus, Z constants
+
+    We also define a relation symbol for my_In.
+
+    Our functions and relations have dependent types; functions are indexed by the argument types and return type,
+    and relations are indexed by the argument types. The argument types are encoded as a list of fol_sorts symbols.
+  
+  *)
 
 
-  Notation sig' := (UF.sig sig symbs).
+  Inductive fol_list_funs : list fol_sorts -> fol_sorts -> Type := 
+    | nil_f : fol_list_funs [] sort_lA
+    | cons_f : fol_list_funs [sort_A; sort_lA] sort_lA
+    | my_app_f : fol_list_funs [sort_lA; sort_lA] sort_lA
+    | my_rev_f : fol_list_funs [sort_lA] sort_lA
+    | tail_rev_f : fol_list_funs [sort_lA; sort_lA] sort_lA
+    | my_len_f : fol_list_funs [sort_lA] sort_Z
+    | plus_f : fol_list_funs [sort_Z; sort_Z] sort_Z
+    | z_const_f : forall (z: Z), fol_list_funs [] sort_Z.
 
-  Require Import MirrorSolve.Reflection.Core.
-  Require Import MirrorSolve.Reflection.FM.
-  Require Import MirrorSolve.Reflection.Tactics.
+  Inductive fol_list_rels : list fol_sorts -> Type := 
+    | my_In_r : fol_list_rels [sort_A; sort_lA].
 
-  MetaCoq Quote Definition t_app := @app.
-  MetaCoq Quote Definition t_rev := @my_rev.
-  MetaCoq Quote Definition t_tail_app := @tail_app.
+  (* We package these up into a first-order logic *signature* for lists: the type symbols + function + relation symbols. 
+  
+  *)
+
+  Definition list_sig: signature := {| 
+    sig_sorts := fol_sorts;
+    sig_funs := fol_list_funs;
+    sig_rels := fol_list_rels 
+  |}.
+
+  (* Next we give a semantics to the function and relation symbols, in terms of the original functions and relation.
+    We use equations because the semantics has a dependent type (the sort symbols are interpreted for arguments and results).
+    The interpreted arguments are provided in a HList input.
+  *)
+
+  Equations interp_fun args ret (f: fol_list_funs args ret) (hargs : HList.t interp_sorts args) : interp_sorts ret := {
+    interp_fun _ _ nil_f _ := nil;
+    interp_fun _ _ cons_f (x ::: l ::: hnil):= x :: l;
+    interp_fun _ _ my_app_f (l ::: r ::: hnil):= my_app l r;
+    interp_fun _ _ my_rev_f (x ::: hnil) := my_rev x;
+    interp_fun _ _ tail_rev_f (x ::: l ::: hnil) := tail_rev x l;
+    interp_fun _ _ my_len_f (x ::: hnil) := my_len x;
+    interp_fun _ _ plus_f (l ::: r ::: hnil) := (l + r)%Z;
+    interp_fun _ _ (z_const_f z) hnil := z;
+  }.
+  
+  Equations interp_rel args (r: fol_list_rels args) (hargs : HList.t interp_sorts args) : Prop := {
+    interp_rel _ my_In_r (x ::: l ::: hnil)  := my_In x l;
+  }.
+
+  (* We can wrap these definitions together with the previous signature to get a first-order logic *model* for mirrorsolve! *)
+
+  Program Definition fm_model : model list_sig := {|
+    FirstOrder.mod_sorts := interp_sorts;
+    FirstOrder.mod_fns := interp_fun;
+    FirstOrder.mod_rels := interp_rel;
+  |}.
+
+
+  (* Next we configure the reflection logic for mirrorsolve. 
+    So we're going to connect the first-order logic syntax and semantics with Coq's AST in MetaCoq. 
+  *)
+
+  (* First we use MetaCoq to get quoted ASTs for the function symbols.
+     If a term has implicit arguments (such as nil: forall A, list A),
+     we need to quote a coq term that *doesn't* have implicits (for example @nil).
+     A safe rule of thumb is to use @ before every quoted term.
+  *)
 
   MetaCoq Quote Definition t_cons := @cons.
   MetaCoq Quote Definition t_nil := @nil.
+  MetaCoq Quote Definition t_my_app := @my_app.
+  MetaCoq Quote Definition t_my_rev := @my_rev.
+  MetaCoq Quote Definition t_tail_rev := @tail_rev.
+  MetaCoq Quote Definition t_my_len := @my_len.
+  MetaCoq Quote Definition t_plus := @Z.add.
+  MetaCoq Quote Definition t_my_In := @my_In.
 
-  (* Some match tactics for the meta-interpreter. 
-    The meta-interpreter converts these definitions into a reflection procedure between pure Coq goals and FOL terms in the UF + Lists combined theory. 
+  (* z constants are handled by a mirrorsolve primitive *)
+
+  (* Next we need boolean tests for checking whether a metacoq AST term is a particular quoted value *)
+  Definition is_t_cons t :=  eq_ctor t t_cons.
+  Definition is_t_nil t :=  eq_ctor t t_nil.
+  Definition is_t_my_app t :=  eq_ctor t t_my_app.
+  Definition is_t_my_rev t :=  eq_ctor t t_my_rev.
+  Definition is_t_tail_rev t :=  eq_ctor t t_tail_rev.
+  Definition is_t_my_len t :=  eq_ctor t t_my_len.
+  Definition is_t_plus t :=  eq_ctor t t_plus.
+  Definition is_t_my_In t :=  eq_term t t_my_In.
+
+  (* We also need to quote the types: Z, A, and list A *)
+  MetaCoq Quote Definition t_Z := (Z).
+  MetaCoq Quote Definition t_lA := (@list A).
+  MetaCoq Quote Definition t_A := (A).
+  MetaCoq Quote Definition t_bool := (bool).
+  
+
+  (* Next we have some machinery for reflecting between normal Coq goals and goals in FOL,
+    and we start with some helper notation for calling mirrorsolve conversion functions. 
+     Plain function and relation symbols are easy so mirrorsolve can auto-generate reflection code.
+     More complicated symbols are harder; 
+      for example the function symbol for Z literals is tricky because it quantifies over all Z values.
+     Mirrorsolve has a primitive for converting Z constants which we use here.
+   *)
+
+  Require Import MirrorSolve.Reflection.Tactics.
+
+  Notation tac_fun_list f := (tac_fun list_sig f).
+  Notation tac_rel_list f := (tac_rel list_sig f).
+
+  (* This line is really tricky to understand, I wouldn't puzzle through the details unless you're really curious! *)
+  Notation tac_z_list := (tacLit list_sig fm_model z_lit (fun x => (sort_Z; x)) (fun x _ => (sort_Z; TFun list_sig (z_const_f x) hnil)) ltac:(solve_lit_wf)).
+
+  (* List of reflection matches; the first element is a test function and the second is a conversion tactic to apply.
+   *)
+  Definition match_tacs : list ((term -> bool) * tac_syn list_sig fm_model) := [
+      ( is_t_my_In, tac_rel_list my_In_r)
+    ; ( is_t_cons, tac_fun_list cons_f)
+    ; ( is_t_nil, tac_fun_list nil_f)
+    ; ( is_t_my_app, tac_fun_list my_app_f)
+    ; ( is_t_my_rev, tac_fun_list my_rev_f)
+    ; ( is_t_tail_rev, tac_fun_list tail_rev_f)
+    ; ( is_t_my_len, tac_fun_list my_len_f)
+    ; ( is_t_plus, tac_fun_list plus_f)
+    ; ( is_z_term, tac_z_list )
+  ].
+
+  (* Analogous reflection matches for sorts *)
+  Definition match_inds : list ((term -> bool) * fol_sorts) := [
+      (eq_term t_lA, sort_lA)
+    ; (eq_term t_A, sort_A)
+    ; (eq_term t_Z, sort_Z)
+    ; (eq_term t_bool, sort_bool)
+  ].
+
+  (* Next we configure the backend SMT plugin. *)
+
+  Declare ML Module "mirrorsolve".
+
+  (* The section variable A is an uninterpreted sort in SMT. *)
+  RegisterCustomSort sort_A "A".
+
+  (*  The inductive sort list A maps to an inductive smt sort,
+      specified as a sum (coq list) of products (also a coq list),
+      with cons and nil constructors.
+  *)
+  RegisterSMTInd sort_lA (SICases [
+      ("cons"%string, [SISort (SCustom "A"); SIRec]) (* This declares an smt constructor named cons with an "A" argument and a recursive argument (i.e. the inner list) *)
+    ; ("nil"%string, []) (* This declares an smt constructor named nil with no arguments *)
+  ]) "A_list".
+
+  (* Map the Z sort to SMT Int, and the bool sort to SMT bool *)
+  RegisterSMTSort sort_Z SInt.
+  RegisterSMTSort sort_bool SBool.
+
+  (* The inductive declaration puts "cons" and "nil" in scope as SMT function symbols, 
+    but the rest of our functions/relations still need to be declared. 
+    We do this with the RegisterSMTUF vernacular. 
+    The syntax for this vernacular is:
+
+    RegisterSMTUF "<function name>" return_sort argument_sorts.
+
+    Where argument_sorts is a list of sort syntaxes. 
+    It's reversed to make parsing the vernacular easier.
   *)
 
-  Definition is_cons t :=
-    match t with 
-    | tApp f _ => eq_term t_cons f
-    | _ => false
-    end.
+  RegisterSMTUF "my_app" sort_lA sort_lA sort_lA.
+  RegisterSMTUF "my_rev" sort_lA sort_lA.
+  RegisterSMTUF "my_len" sort_Z sort_lA.
+  RegisterSMTUF "tail_rev" sort_lA sort_lA sort_lA.
+  RegisterSMTUF "my_In" sort_bool sort_A sort_lA.
 
-  Definition is_nil t :=
-    match t with 
-    | tApp f _ => eq_term t_nil f
-    | _ => false
-    end.
+  RegisterSMTFun cons_f "cons" 2.
+  RegisterSMTFun nil_f "nil" 0.
+  RegisterSMTFun my_app_f "my_app" 2.
+  RegisterSMTFun my_rev_f "my_rev" 1.
+  RegisterSMTFun tail_rev_f "tail_rev" 2.
+  RegisterSMTFun my_len_f "my_len" 1.
+  RegisterSMTFun my_In_r "my_In" 2.
+  RegisterSMTFun plus_f "+" 2.
 
-  Definition is_app t := 
-    match t with 
-    | tApp f _ => eq_term t_app f
-    | _ => false
-    end.
-
-  Definition is_rev t := 
-    match t with 
-    | tApp f _ => eq_term t_rev f
-    | _ => false
-    end.
-
-  Definition is_tail_app t := 
-    match t with 
-    | tApp f _ => eq_term t_tail_app f
-    | _ => false
-    end.
-
-  Definition match_tacs : list ((term -> bool) * tac_syn sig' list_uf_model) := [
-      ( is_nil, tacFun _ _ (Mk_fun_sym sig' _ _ (CFun _ symbs nil_f)))
-    ; ( is_cons, tacFun _ _ (Mk_fun_sym sig' _ _ (CFun _ symbs cons_f)))
-    ; ( is_app, tacFun _ _ (Mk_fun_sym sig' _ _ (UFun (s := "app") _ symbs ltac:(solve_uf_membership))))
-    ; ( is_rev, tacFun _ _ (Mk_fun_sym sig' _ _ (UFun (s := "rev") _ symbs ltac:(solve_uf_membership))))
-    ; ( is_tail_app, tacFun _ _ (Mk_fun_sym sig' _ _ (UFun (s := "tail_app") _ symbs ltac:(solve_uf_membership))))
-  ].
-
-  MetaCoq Quote Definition t_sort := (A).
-  MetaCoq Quote Definition list_sort := (list A).
-
-  (* This is an analogous match but for reflecting Coq types into FOL sorts. *)
-  Definition match_inds : list ((term -> bool) * FOList.sorts) := [
-      (eq_term t_sort, TS)
-    ; (eq_term list_sort, LS)
-  ].
-
-
-  Local Declare ML Module "mirrorsolve".
-  RegisterCustomSort TS "A".
-
-  RegisterSMTInd LS (SICases [
-    ("cons"%string, [SISort (SCustom "A"); SIRec]); 
-    ("nil"%string, [])
-    ]) "A_list".
-
-  RegisterSMTUF "app" LS LS LS.
-  RegisterSMTUF "rev" LS LS.
-  RegisterSMTUF "tail_app" LS LS LS.
+  (* Finally we need to handle integer literals *)
+  RegisterSMTBuiltin z_const_f IntLit.
 
   Transparent denote_tm.
-
-  RegisterSMTFun FOList.nil_f "nil" 0.
-  RegisterSMTFun FOList.cons_f "cons" 2.
-
   Require Import MirrorSolve.Axioms.
 
-  Ltac check_goal_sat := 
-    match goal with 
-    | |- ?G => check_interp_pos G; eapply UnsoundAxioms.interp_true
-    end.
   Ltac check_goal_unsat := 
     match goal with 
     | |- ?G => check_unsat_neg G; eapply UnsoundAxioms.interp_true
     end.
 
-  MetaCoq Quote Definition app_app_nil := (
-    (forall (x : A) (xs ys : list A), app (x :: xs) ys = x :: app xs ys) ->
-(forall xs : list A, app [] xs = xs) ->
-forall (a : A) (r : list A), app (app [] [a]) r = app [] (a :: r)
-  ).
+  Create HintDb list_eqns.
 
-  MetaCoq Quote Definition app_app_cons := (
-    (forall (x : A) (xs ys : list A), app (x :: xs) ys = x :: app xs ys) ->
-    (forall xs : list A, app [] xs = xs) ->
-    forall (a a0 : A) (l : list A),
-    (forall r : list A, app (app l [a]) r = app l (a :: r)) ->
-    forall r : list A, app (app (a0 :: l) [a]) r = app (a0 :: l) (a :: r)
-  ).
+  Hint Resolve my_app_equation_1 : list_eqns.
+  Hint Resolve my_app_equation_2 : list_eqns.
+  Hint Resolve my_rev_equation_1 : list_eqns.
+  Hint Resolve my_rev_equation_2 : list_eqns.
+  Hint Resolve tail_rev_equation_1 : list_eqns.
+  Hint Resolve tail_rev_equation_2 : list_eqns.
+  Hint Resolve my_In_equation_1' : list_eqns.
+  Hint Resolve my_In_equation_2' : list_eqns.
+  Hint Resolve my_len_equation_1 : list_eqns.
+  Hint Resolve my_len_equation_2 : list_eqns.
 
-  (* Hammer works for this one *)
+  Ltac prep_proof := 
+    hints_foreach (fun x => pose proof x) "list_eqns";
+    Utils.revert_all;
+    unfold "<->" in *.
+
+  Scheme Equality for fol_sorts.
+
+  Ltac quote_reflect_list := quote_reflect list_sig fm_model fol_sorts_eq_dec match_tacs match_inds.
+  Ltac quote_extract_list := quote_extract list_sig fm_model fol_sorts_eq_dec match_tacs match_inds.
+
+
+  Ltac mirrorsolve :=
+    prep_proof;
+    quote_reflect_list;
+    check_goal_unsat.
+
   Lemma app_app_one : 
     forall (a: A) (l r : list A), 
-      app (app l [a]) r = app l (a :: r).
+      my_app (my_app l [a]) r = my_app l (a :: r).
   Proof.
-    (* induction l; try hammer. *)
-
-    pose proof app_cons.
-    pose proof app_nil. 
-    Utils.revert_all.
-    induction l; Utils.revert_all.
-    
-    - 
-      reflect_goal (UF.sig sig symbs) list_uf_model sorts_eq_dec match_tacs match_inds app_app_nil. 
-      check_goal_unsat.
-    -
-      reflect_goal (UF.sig sig symbs) list_uf_model sorts_eq_dec match_tacs match_inds app_app_cons. 
-      check_goal_unsat.
+    induction l; mirrorsolve.
   Qed.
 
-  MetaCoq Quote Definition app_nil_r_nil := (
-    (forall xs : list A, app [] xs = xs) ->
-(forall (x : A) (xs ys : list A), app (x :: xs) ys = x :: app xs ys) ->
-app [] [] = []
-  ).
+  Hint Immediate app_app_one : list_eqns.
 
-  MetaCoq Quote Definition app_nil_r_cons := (
-    (forall xs : list A, app [] xs = xs) ->
-    (forall (x : A) (xs ys : list A), app (x :: xs) ys = x :: app xs ys) ->
-    forall (a : A) (l : list A), app l [] = l -> app (a :: l) [] = a :: l
-  ).
-
-  (* hammer works for this one *)
-  Lemma app_nil_r : 
-    forall l, app l [] = l.
-  Proof.
-    pose proof app_nil.
-    pose proof app_cons.
-    induction l; Utils.revert_all.
-    - 
-      reflect_goal (UF.sig sig symbs) list_uf_model sorts_eq_dec match_tacs match_inds app_nil_r_nil. 
-      check_goal_unsat.
-    - 
-      reflect_goal (UF.sig sig symbs) list_uf_model sorts_eq_dec match_tacs match_inds app_nil_r_cons. 
-      check_goal_unsat.
-  Qed.
-
-  MetaCoq Quote Definition app_assoc_nil := (
-    (forall xs : list A, app [] xs = xs) ->
-(forall (x : A) (xs ys : list A), app (x :: xs) ys = x :: app xs ys) ->
-(forall l : list A, app l [] = l) ->
-forall ys zs : list A, app (app [] ys) zs = app [] (app ys zs)
-  ).
-
-  MetaCoq Quote Definition app_assoc_cons := (
-    (forall xs : list A, app [] xs = xs) ->
-    (forall (x : A) (xs ys : list A), app (x :: xs) ys = x :: app xs ys) ->
-    (forall l : list A, app l [] = l) ->
-    forall (a : A) (xs : list A),
-    (forall ys zs : list A, app (app xs ys) zs = app xs (app ys zs)) ->
-    forall ys zs : list A, app (app (a :: xs) ys) zs = app (a :: xs) (app ys zs)
-  ).
-
-  (* hammer works for this one *)
   Lemma app_assoc : 
-    forall xs ys zs, app (app xs ys) zs = app xs (app ys zs).
+    forall (x y z: list A),
+      my_app (my_app x y) z = my_app x (my_app y z).
   Proof.
-    pose proof app_nil.
-    pose proof app_cons.
-    pose proof app_nil_r.
-    induction xs; Utils.revert_all.
-    - 
-      reflect_goal (UF.sig sig symbs) list_uf_model sorts_eq_dec match_tacs match_inds app_assoc_nil. 
-      check_goal_unsat.
-    - 
-      reflect_goal (UF.sig sig symbs) list_uf_model sorts_eq_dec match_tacs match_inds app_assoc_cons. 
-      check_goal_unsat.
+    induction x; 
+    mirrorsolve.
   Qed.
 
-  MetaCoq Quote Definition rev_app_nil := (
-    (forall l : list A, app l [] = l) ->
-    my_rev [] = [] ->
-    (forall (x : A) (xs : list A), my_rev (x :: xs) = app (my_rev xs) [x]) ->
-    (forall xs : list A, app [] xs = xs) ->
-    (forall (x : A) (xs ys : list A), app (x :: xs) ys = x :: app xs ys) ->
-    forall r : list A, my_rev (app [] r) = app (my_rev r) (my_rev [])
-  ).
+  Hint Immediate app_assoc : list_eqns.
 
-  MetaCoq Quote Definition rev_app_cons := (
-    (forall xs ys zs : list A, app (app xs ys) zs = app xs (app ys zs)) ->
-    my_rev [] = [] ->
-    (forall (x : A) (xs : list A), my_rev (x :: xs) = app (my_rev xs) [x]) ->
-    (forall xs : list A, app [] xs = xs) ->
-    (forall (x : A) (xs ys : list A), app (x :: xs) ys = x :: app xs ys) ->
-    forall (a : A) (l : list A),
-    (forall r : list A, my_rev (app l r) = app (my_rev r) (my_rev l)) ->
-    forall r : list A, my_rev (app (a :: l) r) = app (my_rev r) (my_rev (a :: l))
-  ).
-  
+  SetSMTSolver "z3".
 
-  (* hammer does not work for the inductive case *)
-  Lemma rev_app : 
-    forall l r, 
-      my_rev (app l r) = app (my_rev r) (my_rev l).
+  Lemma my_rev_app : 
+    forall (l r : list A), 
+     my_rev (my_app l r) = my_app (my_rev r) (my_rev l).
   Proof.
-    (* induction l; try hammer. *)
-    pose proof my_rev_nil.
-    pose proof my_rev_cons.
-    pose proof app_nil.
-    pose proof app_cons.
-    Utils.revert_all.
-    induction l; Utils.revert_all.
-    - 
-      pose proof app_nil_r.
-      Utils.revert_all.
-      reflect_goal (UF.sig sig symbs) list_uf_model sorts_eq_dec match_tacs match_inds rev_app_nil. 
-      check_goal_unsat.
-    - 
-      pose proof app_assoc.
-      Utils.revert_all.
-      reflect_goal (UF.sig sig symbs) list_uf_model sorts_eq_dec match_tacs match_inds rev_app_cons. 
-      check_goal_unsat.
+    induction l;
+    mirrorsolve.
   Qed.
 
-  MetaCoq Quote Definition rev_rev_nil := (
-    my_rev [] = [] ->
-(forall (x : A) (xs : list A), my_rev (x :: xs) = app (my_rev xs) [x]) ->
-(forall xs : list A, app [] xs = xs) ->
-(forall (x : A) (xs ys : list A), app (x :: xs) ys = x :: app xs ys) ->
-my_rev (my_rev []) = []
-  ).
+  Hint Immediate my_rev_app : list_eqns.
 
-  MetaCoq Quote Definition rev_rev_cons := (
-    (forall l r : list A, my_rev (app l r) = app (my_rev r) (my_rev l)) ->
-    (forall xs ys zs : list A, app (app xs ys) zs = app xs (app ys zs)) ->
-    (forall l : list A, app l [] = l) ->
-    my_rev [] = [] ->
-    (forall (x : A) (xs : list A), my_rev (x :: xs) = app (my_rev xs) [x]) ->
-    (forall xs : list A, app [] xs = xs) ->
-    (forall (x : A) (xs ys : list A), app (x :: xs) ys = x :: app xs ys) ->
-    forall (a : A) (l : list A),
-    my_rev (my_rev l) = l -> my_rev (my_rev (a :: l)) = a :: l
-  ).
+  Lemma app_nil_r : 
+    forall l, my_app l [] = l.
+  Proof.
+    induction l; mirrorsolve.
+  Qed.
 
+  Hint Immediate app_nil_r : list_eqns.
 
-  (* hammer works for this one *)
   Lemma rev_rev : 
     forall (l : list A), 
       my_rev (my_rev l) = l.
   Proof.
-    (* induction l; try hammer. *)
-    pose proof my_rev_nil.
-    pose proof my_rev_cons.
-    pose proof app_nil.
-    pose proof app_cons.
-    induction l; Utils.revert_all.
-    - 
-      reflect_goal (UF.sig sig symbs) list_uf_model sorts_eq_dec match_tacs match_inds rev_rev_nil.
-      check_goal_unsat.
-    - 
-      pose proof rev_app.
-      pose proof app_assoc.
-      pose proof app_nil_r.
-      Utils.revert_all.
-      reflect_goal (UF.sig sig symbs) list_uf_model sorts_eq_dec match_tacs match_inds rev_rev_cons.
-      
-      check_goal_unsat.
+    induction l; mirrorsolve.
   Qed.
 
-  MetaCoq Quote Definition tail_app_rev_nil := (
-    (forall acc : list A, tail_app acc [] = acc) ->
-    (forall (acc : list A) (x : A) (xs : list A),
-     tail_app acc (x :: xs) = tail_app (x :: acc) xs) ->
-    my_rev [] = [] ->
-    (forall (x : A) (xs : list A), my_rev (x :: xs) = app (my_rev xs) [x]) ->
-    (forall xs : list A, app [] xs = xs) ->
-    (forall (x : A) (xs ys : list A), app (x :: xs) ys = x :: app xs ys) ->
-    forall acc : list A, tail_app acc [] = app (my_rev []) acc
-  ).
+  Hint Immediate rev_rev : list_eqns.
 
-  MetaCoq Quote Definition tail_app_rev_cons := (
-    (forall l r : list A, my_rev (app l r) = app (my_rev r) (my_rev l)) ->
-    (forall xs ys zs : list A, app (app xs ys) zs = app xs (app ys zs)) ->
-    (forall l : list A, app l [] = l) ->
-    (forall l : list A, my_rev (my_rev l) = l) ->
-    (forall acc : list A, tail_app acc [] = acc) ->
-    (forall (acc : list A) (x : A) (xs : list A),
-     tail_app acc (x :: xs) = tail_app (x :: acc) xs) ->
-    my_rev [] = [] ->
-    (forall (x : A) (xs : list A), my_rev (x :: xs) = app (my_rev xs) [x]) ->
-    (forall xs : list A, app [] xs = xs) ->
-    (forall (x : A) (xs ys : list A), app (x :: xs) ys = x :: app xs ys) ->
-    forall (a : A) (l : list A),
-    (forall acc : list A, tail_app acc l = app (my_rev l) acc) ->
-    forall acc : list A, tail_app acc (a :: l) = app (my_rev (a :: l)) acc
-  ).
- 
-  (* hammer does not work for the inductive case *)
-  Lemma tail_app_rev : 
-    forall (l: list A) acc, 
-      tail_app acc l = app (my_rev l) acc.
+  Lemma tail_rev_spec : 
+    forall (l acc : list A), 
+      tail_rev l acc = my_app (my_rev l) acc.
   Proof.
-    (* induction l; try hammer. *)
-    pose proof tail_app_nil.
-    pose proof tail_app_cons.
-    pose proof my_rev_nil.
-    pose proof my_rev_cons.
-    pose proof app_nil.
-    pose proof app_cons.
-    induction l; Utils.revert_all.
-    - 
-      reflect_goal (UF.sig sig symbs) list_uf_model sorts_eq_dec match_tacs match_inds tail_app_rev_nil.
-      check_goal_unsat.
-    - 
-      pose proof rev_app.
-      pose proof app_assoc.
-      pose proof app_nil_r.
-      pose proof rev_rev.
-      Utils.revert_all.
-      reflect_goal (UF.sig sig symbs) list_uf_model sorts_eq_dec match_tacs match_inds tail_app_rev_cons.
-      check_goal_unsat.
+    induction l; mirrorsolve.
   Qed.
 
-  MetaCoq Quote Definition my_app_sound_term := (
-    (forall acc : list A, tail_app acc [] = acc) ->
-    (forall (acc : list A) (x : A) (xs : list A),
-     tail_app acc (x :: xs) = tail_app (x :: acc) xs) ->
-    my_rev [] = [] ->
-    (forall (x : A) (xs : list A), my_rev (x :: xs) = app (my_rev xs) [x]) ->
-    (forall xs : list A, app [] xs = xs) ->
-    (forall (x : A) (xs ys : list A), app (x :: xs) ys = x :: app xs ys) ->
-    (forall l : list A, my_rev (my_rev l) = l) ->
-    (forall l acc : list A, tail_app acc l = app (my_rev l) acc) ->
-    forall l r : list A, tail_app r (my_rev l) = app l r
-  ).
+  Hint Immediate tail_rev_spec : list_eqns.
 
-  (* hammer works for this one *)
-  Theorem my_app_sound:
-    forall l r,
-      my_app l r = app l r.
+  Lemma tail_rev_sound : 
+    forall (l : list A), 
+      my_rev l = tail_rev l nil.
   Proof.
-    (* unfold my_app; try hammer. *)
-    pose proof tail_app_nil.
-    pose proof tail_app_cons.
-    pose proof my_rev_nil.
-    pose proof my_rev_cons.
-    pose proof app_nil.
-    pose proof app_cons.
-    pose proof rev_rev.
-    pose proof tail_app_rev.
-    Utils.revert_all.
-    unfold my_app.
-    reflect_goal (UF.sig sig symbs) list_uf_model sorts_eq_dec match_tacs match_inds my_app_sound_term.
-    check_goal_unsat.
+    induction l; mirrorsolve.
+  Qed.
+
+  Hint Immediate tail_rev_sound : list_eqns.
+
+  SetSMTSolver "z3".
+
+  Lemma app_len : 
+    forall (l r : list A), 
+      my_len (my_app l r) = (my_len l + my_len r)%Z.
+  Proof.
+    induction l; mirrorsolve.
+  Qed.
+
+  Hint Immediate app_len : list_eqns.
+
+  Lemma rev_len :
+    forall (l: list A), 
+      my_len l = my_len (my_rev l).
+  Proof.
+    induction l; mirrorsolve.
+  Qed.
+  Hint Immediate rev_len : list_eqns.
+
+  Lemma app_In : 
+    forall x l r,
+      my_In x (my_app l r) <-> my_In x l \/ my_In x r.
+  Proof.
+    induction l; mirrorsolve.
+  Qed.
+
+  Hint Immediate app_In : list_eqns.
+  
+  Lemma in_rev : 
+    forall x l,
+      my_In x l <-> my_In x (my_rev l).
+  Proof.
+    induction l; mirrorsolve.
   Qed.
 
 End ListFuncs.
